Correct overflow

EbpfVerifierRangeAnalysis/Overflow.lean
@@ -5,22 +5,58 @@ def UInt_max : UInt64 := UInt64.ofNat (2^64 - 1)
 def Int32_max : Int32 := Int32.maxValue
 def Int_max : Int64 := Int64.maxValue
 
-@[simp]
+
 def unsignedCheckAddOverflow32 (a b : UInt32) : Bool :=
   let sum := a.toNat + b.toNat
-  sum ≥ UInt32_max
+  sum > UInt32_max.toNat
 
 @[simp]
-def signedCheckAddOverflow32 (a b : Int32): Bool :=
-  let sum := a.toNat + b.toNat
-  sum ≥ Int32_max
+theorem unsignedCheckAddOverflow32_iff (a b : UInt32) :
+  unsignedCheckAddOverflow32 a b ↔ a.toNat + b.toNat > 2^32 - 1 := by
+  unfold unsignedCheckAddOverflow32
+  simp
+  unfold UInt32_max
+  simp
+
+
+def signedCheckAddFlows32 (a b : Int32): Bool :=
+  let sum := a.toInt + b.toInt
+  sum > Int32_max.toInt ∨ sum < 0
 
 @[simp]
+theorem signedCheckAddFlows32_iff (a b : Int32):
+  signedCheckAddFlows32 a b ↔
+  (a.toInt + b.toInt > Int32.maxValue.toInt) ∨
+  (a.toInt + b.toInt < 0):= by
+  unfold signedCheckAddFlows32
+  simp
+  unfold Int32_max
+  unfold Int32.maxValue
+  simp
+
 def unsignedCheckAddOverflow(a b : UInt64) : Bool :=
   let sum := a.toNat + b.toNat
-  sum ≥ UInt_max
+  sum > UInt_max.toNat
 
 @[simp]
-def signedCheckAddOverflow (a b : Int64) : Bool :=
-  let sum := a.toNat + b.toNat
-  sum ≥ Int_max
+theorem unsignedCheckAddOverflow_iff (a b : UInt64) :
+  unsignedCheckAddOverflow a b ↔ a.toNat + b.toNat > 2^64 - 1 := by
+  unfold unsignedCheckAddOverflow
+  simp
+  unfold UInt_max
+  simp
+
+def signedCheckAddFlows (a b : Int64) : Bool :=
+  let sum := a.toInt + b.toInt
+  sum > Int_max.toInt ∨ sum < 0
+
+@[simp]
+theorem signedCheckAddOverflow_iff (a b : Int64) :
+  signedCheckAddFlows a b ↔
+  (a.toInt + b.toInt > Int64.maxValue.toInt) ∨
+  (a.toInt + b.toInt < 0) := by
+  unfold  signedCheckAddFlows
+  simp
+  unfold Int_max
+  unfold Int64.maxValue
+  simp
